{
 "cells": [
  {
   "cell_type": "markdown",
   "metadata": {},
   "source": [
    "# Chapter 4. Gaussian Models\n",
    "+ date: 2017-03-20\n",
    "+ tags: mlapp, stat\n",
    "+ author: Peijun Zhu"
   ]
  },
  {
   "cell_type": "markdown",
   "metadata": {},
   "source": [
    "This block is defining some frequently used macros. Removing this block will result in rendering issues.\n",
    "$\\DeclareMathOperator{\\Var}{Var} % Variance\n",
    "\\DeclareMathOperator{\\det}{det} % Determinant\n",
    "\\DeclareMathOperator{\\tr}{tr}   % Trace\n",
    "\\DeclareMathOperator{\\Var}{Var} % Variance\n",
    "\\DeclareMathOperator{\\Var}{Var} % Variance\n",
    "\\DeclareMathOperator{\\Var}{Var} % Variance\n",
    "\\DeclareMathOperator{\\E}{E}     % Expectation\n",
    "\\DeclareMathOperator{\\Cov}{Cov} % Covariance\n",
    "\\DeclareMathOperator{\\Beta}{B}  % Beta function\n",
    "\\DeclareMathOperator{\\Bdist}{Beta}  % Beta distribution\n",
    "\\DeclareMathOperator{\\sgn}{sgn}  % Beta distribution\n",
    "\\DeclareMathOperator{\\adj}{adj}  % Beta distribution\n",
    "\\newcommand{\\pp}{\\partial}      % Partial derivative\n",
    "\\newcommand{\\dd}{\\mathrm{d}}      % Partial derivative\n",
    "\\newcommand{\\pfr}[2]{\\frac{\\pp #1}{\\pp #2}}      % Partial derivative\n",
    "\\newcommand{\\dfr}[2]{\\frac{\\dd #1}{\\dd #2}}      % Total derivative\n",
    "\\newcommand{\\inv}[1]{#1^{-1}}   % Inverse Matrix\n",
    "\\newcommand{\\invt}[1]{#1^{-T}}  % Inverse Transposed Matrix\n",
    "\\DeclareMathOperator{\\ii}{i}    % Imaginary number\n",
    "\\DeclareMathOperator{\\rhs}{RHS}\n",
    "\\DeclareMathOperator{\\lhs}{LHS}\n",
    "\\renewcommand{\\nl}{\\\\&\\phantom{{}={}}}% Newline In aligned equations$"
   ]
  },
  {
   "cell_type": "markdown",
   "metadata": {},
   "source": [
    "## Matrix derivative\n",
    "We are using Einstein's summation rule below: sum over repeating index. It is useful in evaluating matrix/tensor.\n",
    "\n",
    "\\begin{align}\n",
    "\\delta |A|&=|A+\\delta A|-|A|\\\\\n",
    "&=|D+\\inv U\\delta A\\inv V|-|A|\\\\\n",
    "&=|D||I+\\inv A\\delta A|-|A|\\\\\n",
    "&=|A|\\tr(\\inv A\\delta A)\n",
    "\\end{align}\n",
    "\n",
    "Using\n",
    "\n",
    "\\begin{align}\n",
    "\\pfr{|A|}{A}&=e_ie_j^T\\pfr{|A|}{A_{ij}}\\\\\n",
    "&=e_ie_j^T|A|\\tr(\\inv A\\pfr{A}{A_{ij}})\\\\\n",
    "&=e_ie_j^T|A|\\tr(\\inv Ae_ie_j)\\\\\n",
    "&=e_ie_j^T|A|\\inv A_{ji}\\\\\n",
    "&=|A|\\invt A\n",
    "\\end{align}\n",
    "\n",
    "$$\\pfr{A_{ij}B_{ji}}{A}=e_me_n^T\\pfr{A_{ij}B_{ji}}{A_{mn}}=B_{nm}e_me_n^T=B^T$$\n",
    "\n",
    "$$\\pfr{a^TAa}{a}=e_m\\pfr{a_iA_{ij}a_j}{a_m}=e_m(A_{mj}a_j+a_i A_{im})=(A+A^T)a$$\n",
    "\n",
    "$$\\pfr{a^TAa}{A}=e_me_n^T\\pfr{a_iA_{ij}a_j}{A_{mn}}=aa^T$$\n",
    "\n",
    "$$\\pfr{\\tr AB}{A}=e_me_n^T\\pfr{A_{ij}B_{ji}}{A_{mn}}=e_me_n^TB_{nm}=B^T$$\n",
    "\n",
    "Using these relationships, it is straightforward to MLE"
   ]
  },
  {
   "cell_type": "markdown",
   "metadata": {
    "collapsed": true
   },
   "source": [
    "## Maximal Entropy of Gaussian Dist from Variation\n",
    "Consider entropy\n",
    "\n",
    "\\begin{align}\n",
    "S&=-\\int p\\ln p \\dd V-a\\left(\\int p\\dd V-1\\right)-\\sum_i b_i\\left(\\int x_ip\\dd V\\right)\\nl-\\sum_{i,j} C_{ij}\\left(\\int x_ix_jp\\dd V-\\Sigma_{ij}\\right)\\\\\n",
    "&=-\\int (\\ln p+a+b^Tx+x^TCx)p \\dd V+a+\\tr(C\\Sigma)\\\\\n",
    "&=-\\int L(p,x)\\dd x+a+c\n",
    "\\end{align}\n",
    "\n",
    "The Euler-Lagrange equation is\n",
    "\n",
    "\\begin{align}\n",
    "\\pfr{L}{p}&=1+a+b^Tx+x^TCx+\\ln p=0\\\\\n",
    "\\Rightarrow p(x)&=\\exp(-1-a-b^Tx-x^TCx)\n",
    "\\end{align}\n",
    "\n",
    "It is a Gaussian distribution, with constraints:\n",
    "\n",
    "\\begin{align}\n",
    "\\int p\\dd V&=1\\\\\n",
    "\\int x_ip\\dd V&=0\\\\\n",
    "\\int x_ix_jp\\dd V&=\\Sigma_{ij}\\\\\n",
    "\\end{align}\n",
    "\n",
    "and we can determine $a,b,c$ from constraints. Multivariable case is harder, but the method is the same: using multiplier and EL equation. "
   ]
  },
  {
   "cell_type": "markdown",
   "metadata": {
    "collapsed": true
   },
   "source": [
    "## Sigmoid model\n",
    "$$\\exp\\left[\\frac{(x-\\mu)^2}{2\\sigma^2}\\right]=\\exp\\left(\\frac{x^2+\\mu^2-2\\mu x}{2\\sigma^2}\\right)=Af(x)\\exp(\\mu x/\\sigma^2)$$\n",
    "$$\\frac{A\\exp(ax)}{A\\exp(ax)+B\\exp(bx)}=\\frac{1}{1+\\exp(Dx+C)}$$"
   ]
  },
  {
   "cell_type": "markdown",
   "metadata": {},
   "source": [
    "# Exercises"
   ]
  },
  {
   "cell_type": "markdown",
   "metadata": {},
   "source": [
    "## 4.1\n",
    "As\n",
    "$$\\E[x]=0,\\quad \\E[y]=\\E[x]^2+\\Var[x]^2=1/3$$\n",
    "\n",
    "\\begin{align}\n",
    "\\Cov[x,y]&=E[xy-x\\bar y-\\bar xy+\\bar x\\bar y]\\\\\n",
    "&=\\E[xy]-\\E[x]\\E[y]\\\\\n",
    "&=\\int_{-1}^1 \\frac{x^3}{2}dx\\\\\n",
    "&=0\\\\\n",
    "&\\Rightarrow\\rho=0\\end{align}"
   ]
  },
  {
   "cell_type": "markdown",
   "metadata": {
    "collapsed": true
   },
   "source": [
    "# 4.2\n",
    "$$P(Y=y)=\\frac{P(X=y)+P(X=-y)}{2}=P(X=y)$$\n",
    "It is obvious that $\\E[x]=\\E[y]=0$,\n",
    "\n",
    "\\begin{align}\n",
    "\\Cov[x,y]&=\\E[xy]-\\E[x]\\E[y]\\\\\n",
    "&=P(W=1)\\E[x,y|W=1]+P(W=-1)\\E[x,y|W=-1]\\\\\n",
    "&=(E[x^2]+E[-x^2])/2\\\\\n",
    "&=0\n",
    "\\end{align}"
   ]
  },
  {
   "cell_type": "markdown",
   "metadata": {},
   "source": [
    "# 4.3\n",
    "We need to prove $|\\rho|<1$, i.e. \n",
    "$$\\Cov[x,y]^2\\leq \\Cov[x,x]\\Cov[y,y]$$\n",
    "\n",
    "The $\\Cov$ function satisty\n",
    "+ Symmetry $\\Cov[x,y]=\\Cov[y,x]$\n",
    "+ Double linearity $\\Cov[\\lambda x+\\mu y, z]=\\lambda\\Cov[x, z]+\\mu\\Cov[y,z]$\n",
    "+ Positive definiteness $\\Cov[x, x]\\geq 0$, equal sign holds iff $x=0$\n",
    "\n",
    "Using Cauchy-Schwartz Inequality, the conclusion is straightforward."
   ]
  },
  {
   "cell_type": "markdown",
   "metadata": {},
   "source": [
    "# 4.4\n",
    "It is obvious that $\\Cov[X,Y+c]=\\Cov[X,Y]$ for any const $c$. So for $Y=aX+b$, \n",
    "\n",
    "\\begin{align}\n",
    "\\Cov[X,Y]&=\\Cov[x,aX]=a\\Cov[x,x]\\\\\n",
    "\\Cov[Y,Y]&=a^2\\Cov[X,X]\n",
    "\\end{align}\n",
    "\n",
    "So we have\n",
    "$$\\rho=\\frac{\\Cov[X,Y]}{\\sqrt{\\Cov[X,X]\\Cov[Y,Y]}}=\\frac{a\\Cov[X,X]}{|a|\\Cov[X,X]}=\\sgn[a]$$"
   ]
  },
  {
   "cell_type": "markdown",
   "metadata": {},
   "source": [
    "# 4.5\n",
    "Suppose $\\Lambda=\\Sigma^{-1}=U^TDU$, where $U$ is orthonormal and $D$ is diagonal, then we can find basis $\\vec y=U(\\vec x-\\vec{\\mu})$ , which simplifies the integral to\n",
    "\n",
    "\\begin{align}\n",
    "\\int \\exp\\left(-\\frac{y^TDy}{2}\\right)&=\\prod \\int \\exp\\left(-\\frac{D_iy_i^2}{2}\\right)dy_i\\\\\n",
    "&=\\prod \\sqrt{\\frac{2\\pi}{D_i}}\\\\\n",
    "&=\\frac{(2\\pi)^{d/2}}{\\sqrt{\\det D}}\\\\\n",
    "&=(2\\pi)^{d/2}\\sqrt{\\det \\Sigma}\\\\\n",
    "\\end{align}"
   ]
  },
  {
   "cell_type": "markdown",
   "metadata": {},
   "source": [
    "# 4.6\n",
    "Obviously, $\\det\\Sigma=(1-\\rho^2)\\sigma_1^2\\sigma_2^2$\n",
    "\n",
    "The inverse matrix of $\\Sigma$ is \n",
    "\n",
    "\\begin{align}\n",
    "\\Lambda&=\\adj\\Sigma/\\det\\Sigma\\\\\n",
    "&=\\begin{bmatrix}\n",
    "\\sigma_2^2& -\\rho\\sigma_1\\sigma_2\\\\\n",
    "-\\rho\\sigma_1\\sigma_2& \\sigma_1^2\n",
    "\\end{bmatrix}/\\left[(1-\\rho^2)\\sigma_1^2\\sigma_2^2\\right]\\\\\n",
    "&=\\frac{1}{1-\\rho^2}\\begin{bmatrix}\n",
    "\\dfrac{1}{\\sigma_1^2}& -\\dfrac{\\rho}{\\sigma_1\\sigma_2}\\\\\n",
    "-\\dfrac{\\rho}{\\sigma_1\\sigma_2}& \\dfrac{1}{\\sigma_2^2}\n",
    "\\end{bmatrix}\n",
    "\\end{align}\n",
    "Plug thess expressions into the original pdf, we can easily prove the (4.268) "
   ]
  },
  {
   "cell_type": "markdown",
   "metadata": {},
   "source": [
    "# 4.7 Bivariate conditioning\n",
    "\\begin{align}\n",
    "p(x_1,x_2)&=\\frac{1}{2\\pi\\sigma_1\\sigma_2\\sqrt{1-\\rho^2}}\\exp\\left(-\\frac{1}{2(1-\\rho^2)}\\left(\\frac{(x_1-\\mu_1)^2}{\\sigma_1^2}+\\frac{(x_2-\\mu_2)^2}{\\sigma_2^2}-2\\rho \\frac{x_1-\\mu_1}{\\sigma_1}\\frac{x_2-\\mu_2}{\\sigma_2}\\right)\\right)\\\\\n",
    "& =\\frac{1}{2\\pi\\sigma_1\\sigma_2\\sqrt{1-\\rho^2}}\\exp\\left(-\\frac{1}{2(1-\\rho^2)}\\left(\\frac{x_1-\\mu_1}{\\sigma_1}-\\rho\\frac{x_2-\\mu_2}{\\sigma_2}\\right)^2+\\frac{(x_2-\\mu_2)^2}{2\\sigma_2^2}\\right)\\\\\n",
    "& =\\frac{N(x_2|\\mu_2,\\sigma_2^2)}{\\sqrt{2\\pi}\\sigma_1\\sqrt{1-\\rho^2}}\\exp\\left(-\\frac{1}{2\\sigma_1^2(1-\\rho^2)}\\left(x_1-\\mu_1-\\rho\\frac{\\sigma_1}{\\sigma_2}(x_2-\\mu_2)\\right)^2\\right)\\\\\n",
    "&=N(x_2|\\mu_2,\\sigma_2^2)N\\left(x_1\\Big|\\mu_1+\\rho\\frac{\\sigma_1}{\\sigma_2}(x_2-\\mu_2),\\sigma_1^2(1-\\rho^2)\\right)\\\\\n",
    "&=p(x_2)N\\left(x_1\\Big|\\mu_1+\\rho\\frac{\\sigma_1}{\\sigma_2}(x_2-\\mu_2),\\sigma_1^2(1-\\rho^2)\\right)\\\\\n",
    "\\Rightarrow\\quad p(x_1|x_2)&=N\\left(x_1\\Big|\\mu_1+\\rho\\frac{\\sigma_1}{\\sigma_2}(x_2-\\mu_2),\\sigma_1^2(1-\\rho^2)\\right)\n",
    "\\end{align}\n",
    "\n",
    "If $\\sigma_i=1$, then it is simplified to\n",
    "$$p(x_1|x_2)=N\\left(x_1|\\mu_1+\\rho(x_2-\\mu_2),1-\\rho^2\\right)$$"
   ]
  },
  {
   "cell_type": "markdown",
   "metadata": {},
   "source": [
    "# 4.8 TBD\n",
    "Try to use python to solve it!"
   ]
  },
  {
   "cell_type": "markdown",
   "metadata": {},
   "source": [
    "# 4.9 Sensor fusion with known variances in 1d\n",
    "\\begin{align}\n",
    "p(\\mu|D)&\\propto \\prod_i N(y_i^{(1)}|\\mu, v_1)\\prod_i N(y_i^{(2)}|\\mu, v_2)\\\\\n",
    "&\\propto \\prod_i N(\\mu|y_i^{(1)}, v_1)\\prod_i N(\\mu|y_i^{(2)}, v_2)\\\\\n",
    "&\\propto \\prod_i N_c(\\mu|v_1^{-1}y_i^{(1)}, v_1^{-1})\\prod_i N_c(\\mu|v_2^{-1}y_i^{(2)}, v_2^{-1})\\\\\n",
    "&\\propto N_c\\left(\\mu\\Big|v_1^{-1}\\sum_i y_i^{(1)}+v_2^{-1}\\sum_i y_i^{(2)}, n_1v_1^{-1}+n_2v_2^{-1}\\right)\\\\\n",
    "&\\propto N_c\\left(\\mu\\Big|n_1v_1^{-1}\\bar y^{(1)}+n_2v_2^{-1}\\bar y^{(2)}, n_1v_1^{-1}+n_2v_2^{-1}\\right)\\\\\n",
    "&\\propto N\\left(\\mu\\Big|\\frac{n_1\\bar y^{(1)}/v_1+n_2\\bar y^{(2)}/v_1}{n_1/v_1+n_2/v_2}, \\frac{1}{n_1/v_1+n_2/v_2}\\right)\n",
    "\\end{align}\n",
    "\n",
    "So the mean of $\\mu$ is $\\dfrac{n_1\\bar y^{(1)}/v_1+n_2\\bar y^{(2)}/v_1}{n_1/v_1+n_2/v_2}$, and variance of $\\mu$ is $\\dfrac{1}{n_1/v_1+n_2/v_2}$."
   ]
  },
  {
   "cell_type": "markdown",
   "metadata": {
    "collapsed": true
   },
   "source": [
    "# 4.10 Information form marginalization formula\n",
    "$$\\det \\Lambda=\\det \\Sigma^{-1}=(\\det\\Sigma)^{-1}$$\n",
    "\n",
    "\\begin{align}\n",
    "(x-\\mu)^T\\Sigma^{-1}(x-\\mu)&=x^T\\Lambda x-2x^T\\Lambda \\mu+\\mu^T\\Lambda\\mu\\\\\n",
    "&=x^T\\Lambda x-2x^T\\xi+\\xi^T\\Lambda^{-1}\\xi\n",
    "\\end{align}\n",
    "\n",
    "From $$\\begin{bmatrix}\n",
    "\\Sigma_{11}& \\Sigma_{12}\\\\\n",
    "\\Sigma_{21}& \\Sigma_{22}\n",
    "\\end{bmatrix}\n",
    "\\cdot\\begin{bmatrix}\n",
    "\\Lambda_{11}&\\Lambda_{12}\\\\\n",
    "\\Lambda_{21}&\\Lambda_{22}\n",
    "\\end{bmatrix}=I,$$\n",
    "we find \n",
    "\n",
    "\\begin{align}\n",
    "\\Sigma_{11}^{-1}=\\Lambda_{11}-\\Lambda_{12}\\Lambda_{22}^{-1}\\Lambda_{21},\\quad \\Sigma_{12}^{-1}=\\Lambda_{21}-\\Lambda_{22}\\Lambda_{12}^{-1}\\Lambda_{11}\\\\\n",
    "\\Sigma_{21}^{-1}=\\Lambda_{12}-\\Lambda_{11}\\Lambda_{21}^{-1}\\Lambda_{22},\\quad \\Sigma_{22}^{-1}=\\Lambda_{22}-\\Lambda_{21}\\Lambda_{11}^{-1}\\Lambda_{12}\n",
    "\\end{align}\n",
    "\n",
    "Using the rule $N(\\mu,\\Sigma)\\rightarrow N_c(\\Sigma^{-1}\\mu,\\Sigma^{-1})$\n",
    "\n",
    "\\begin{align}\n",
    "p(x_2)&=N(x_2|\\mu_2,\\Sigma_{22})\\\\\n",
    "&=N_c(x_2|\\Sigma_{22}^{-1}\\mu_2, \\Sigma_{22}^{-1})\\\\\n",
    "&=N_c(x_2|(\\Lambda_{22}-\\Lambda_{21}\\Lambda_{11}^{-1}\\Lambda_{12})\\mu_2,\\Sigma_{22}^{-1})\\\\\n",
    "&=N_c(x_2|(\\Lambda_{22}\\mu_2+\\Lambda_{21}\\mu_1)-\\Lambda_{21}\\Lambda_{11}^{-1}(\\Lambda_{11}\\mu_1+\\Lambda_{12}\\mu_2),\\Sigma_{22}^{-1})\\\\\n",
    "&=N_c(x_2|\\xi_2-\\Lambda_{21}\\Lambda_{11}^{-1}\\xi_1,\\Lambda_{22}-\\Lambda_{21}\\Lambda_{11}^{-1}\\Lambda_{12})\\\\\n",
    "p(x_1|x_2)&=N(x_1|\\mu_{1|2}, \\Sigma_{1|2})\\\\\n",
    "&=N(x_1|\\Lambda_{11}^{-1}(\\Lambda_{11}\\mu_1-\\Lambda_{12}(x_2-\\mu_2)), \\Lambda_{11}^{-1})\\\\\n",
    "&=N_c(x_1|\\Lambda_{11}\\mu_1-\\Lambda_{12}(x_2-\\mu_2),\\Lambda_{11})\\\\\n",
    "&=N_c(x_1|(\\Lambda_{11}\\mu_1+\\Lambda_{12}\\mu_2)-\\Lambda_{12}x_2,\\Lambda_{11})\\\\\n",
    "&=N_c(x_1|\\xi_1-\\Lambda_{12}x_2,\\Lambda_{11})\\\\\n",
    "\\end{align}"
   ]
  },
  {
   "cell_type": "markdown",
   "metadata": {},
   "source": [
    "# Linear Gaussian system\n",
    "\\begin{align}\n",
    "p(x)&=N(x|\\mu_x, \\Sigma_x)\\\\\n",
    "p(y|x)&=N(y|Ax+b,\\Sigma_y)\n",
    "\\end{align}\n",
    "As $y=Ax+b$, we find $x=A^{-1}(y-b)$, so $$(y-Ax-b)^T\\Sigma_y(y-Ax-b)=[x-A^{-1}(y+b)]^TA^T\\Sigma_y^{-1}A[x-A^{-1}(y+b)]$$\n",
    "Thus\n",
    "\n",
    "\\begin{align}\n",
    "N(y|Ax+b,\\Sigma_y)&=N\\left(x|A^{-1}(y-b), A^{-1}\\Sigma_yA^{-T}\\right)\\\\\n",
    "&=N_c(x|A^T\\Sigma_y^{-1}AA^{-1}(y-b), A^T\\Sigma_y^{-1}A)\\\\\n",
    "&=N_c(x|A^T\\Sigma_y^{-1}(y-b), A^T\\Sigma_y^{-1}A)\\\\\n",
    "&=N_c(y|\\Sigma_y^{-1}(Ax+b), \\Sigma_y^{-1})\n",
    "\\end{align}\n",
    "\n",
    "\\begin{align}\n",
    "p(x,y)&= N(x|\\mu_x, \\Sigma_x)N(y|Ax+b,\\Sigma_y)\\\\\n",
    "&=N_c(x|\\Sigma_x^{-1}\\mu_x, \\Sigma_x^{-1})N_c(x|A^T\\Sigma_y^{-1}(y-b), A^T\\Sigma_y^{-1}A)\\\\\n",
    "&=p(y)N_c(x|\\Sigma_x^{-1}\\mu_x+A^T\\Sigma_y^{-1}(y-b), \\Sigma_x^{-1}+A^T\\Sigma_y^{-1}A)\\\\\n",
    "&=p(y)N(x|\\mu_{x|y},\\Sigma_{x|y})\\\\\n",
    "&=p(y)p(x|y)\\\\\n",
    "\\end{align}\n",
    "Where\n",
    "\n",
    "\\begin{align}\n",
    "\\Sigma_{x|y}^{-1}&=\\Sigma_x^{-1}+A^T\\Sigma_y^{-1}A\\\\\n",
    "\\mu_{x|y}&=\\Sigma_{x|y}[\\Sigma_x^{-1}\\mu_x+A^T\\Sigma_y^{-1}(y-b)]\\end{align}\n",
    "How to calculate $p(y)$?\n",
    "### Attempt\n",
    "We can rewrite \n",
    "$$N_c(x|A^T\\Sigma_y^{-1}y+(A^T\\Sigma_y^{-1}b+\\Sigma_x^{-1}\\mu_x), \\Sigma_x^{-1}+A^T\\Sigma_y^{-1}A)=N_c(y|Cx+d, xx)$$\n",
    "From $p(x,y)=p(y)p(x|y)$, we find $\\Sigma^{-1}=\\Sigma_x^{-1}+A^T\\Sigma_y^{-1}A-\\Sigma_{x|y}^{-1}$"
   ]
  },
  {
   "cell_type": "markdown",
   "metadata": {},
   "source": [
    "## 11ï¼Œ12\n",
    "## 13\n",
    "$$p(\\mu|D)\\propto N(\\mu|\\mu_0,9)\\prod_i N(y_i|\\mu, 4)$$\n",
    "And we find $\\mu\\sim N(\\mu_n,\\sigma_n^2)$, where $\\sigma_n^2=\\dfrac{1}{1/9+n/4}$, so $n=4/\\sigma_n^2-4/9$. We need\n",
    "$$1.96\\sigma_n=1/2\\quad\\Rightarrow n>62.29$$"
   ]
  }
 ],
 "metadata": {
  "kernelspec": {
   "display_name": "Python 3",
   "language": "python",
   "name": "python3"
  },
  "language_info": {
   "codemirror_mode": {
    "name": "ipython",
    "version": 3
   },
   "file_extension": ".py",
   "mimetype": "text/x-python",
   "name": "python",
   "nbconvert_exporter": "python",
   "pygments_lexer": "ipython3",
   "version": "3.6.0"
  }
 },
 "nbformat": 4,
 "nbformat_minor": 2
}
